%!TEX root = main.tex

\section{Aufgabe 2 Bernstein-Bezier-Darstellung}

\subsection*{a)}



$\xi = 1$


\begin{tabular}{cccc}
\vect{1\\5} &   \multirow{3}{*}{\vect{1\\3}}& \multirow{5}{*}{\vect{2\\2}} &\multirow{7}{*}{\vect{3.5\\2}}\\ 
\vect{1\\1} &   \multirow{3}{*}{\vect{3\\1}}& \multirow{6}{*}{\vect{5\\2}} &\\ 
\vect{5\\1} &   \multirow{3}{*}{\vect{7\\3}}&  & \\ 
\vect{9\\5} &   &  &\\
\end{tabular}

\bigskip

$\xi = 3$

\begin{tabular}{cccc}
 \vect{1\\5} &  \multirow{3}{*}{\vect{1\\-1}}& \multirow{5}{*}{\vect{10\\2}} &\multirow{7}{*}{\vect{14.5\\14}}\\ 
 \vect{1\\1} &  \multirow{3}{*}{\vect{7\\1}}& \multirow{6}{*}{\vect{13\\10}} &\\ 
 \vect{5\\1} &  \multirow{3}{*}{\vect{11\\7}}&  & \\ 
 \vect{9\\5} &   &  &\\
\end{tabular}


\bigskip


\input{plot}


\subsection*{b)}

\begin{equation}
{\bf P}(t) = \vect{1\\5} \text{B}_{30}(t) + \vect{1\\3} \text{B}_{21}(t) + \vect{2\\2} \text{B}_{12}(t) + \vect{3.5\\2} \text{B}_{03}(t) , t \in [0,1]
\end{equation}


\begin{equation}
{\bf P}(t) = \vect{3.5\\2} \text{B}_{30}(t) + \vect{5\\2} \text{B}_{21}(t) + \vect{7\\3} \text{B}_{12}(t) + \vect{9\\5} \text{B}_{03}(t) , t \in [1,2]
\end{equation}

\begin{equation}
{\bf P}(t) = \vect{1\\5} \text{B}_{30}(t) + \vect{1\\-1} \text{B}_{21}(t) + \vect{10\\2} \text{B}_{12}(t) + \vect{14.5\\14} \text{B}_{03}(t) , t \in [0,3]
\end{equation}

\begin{equation}
{\bf P}(t) = \vect{9\\5} \text{B}_{30}(t) + \vect{11\\7} \text{B}_{21}(t) + \vect{13\\10} \text{B}_{12}(t) + \vect{14.5\\14} \text{B}_{03}(t) , t \in [2,3]
\end{equation}


\subsection*{c)}

\begin{equation}
{\bf P}(1) = \vect{3.5\\2} 
\end{equation}

\begin{equation}
{\bf P}'(1) = \frac{3}{2} \left( \vect{2\\2} - \vect{5\\2} \right) =  \vect{ -\frac{9}{2}\\2} 
\end{equation}

\begin{equation}
{\bf P}''(1) = \frac{3}{2} \left( \vect{7\\3} - 2 \vect{3\\1} + \vect{1\\3} \right) =  \vect{ 3 \\ 6} 
\end{equation}

\begin{equation}
{\bf P}'''(1) = \frac{3}{2} \left( - \vect{1\\5} + 3 \vect{1\\1} - 3 \vect{5\\1} + \vect{9\\5} \right) =  \vect{ - 6 \\ 6} 
\end{equation}

\begin{equation}
{\bf P}(3) = \vect{14.5\\14} 
\end{equation}

\begin{equation}
{\bf P}'(3) = \frac{3}{2} \left( \vect{13\\10} - \vect{10\\2} \right) =  \vect{ -\frac{9}{2}\\ 12} 
\end{equation}

\begin{equation}
{\bf P}''(3) = \frac{3}{2} \left( \vect{1\\-1} - 2 \vect{7\\1} + \vect{11\\7} \right) =  \vect{ -3 \\ 6} 
\end{equation}

\begin{equation}
{\bf P}'''(3) = \frac{3}{2} \left( - \vect{1\\5} + 3 \vect{1\\1} - 3 \vect{5\\1} + \vect{9\\5} \right) =  \vect{ - 6 \\ 6} 
\end{equation}








